extract/TestSwap.v
@@ -1,0 +1,11 @@
+From Extract Require Import
+     IO_Test.
+From App Require Import
+     Execute.
+Extraction Blacklist Char.
+
+Definition run_test : io_unit :=
+  IO.unsafe_run
+    (ORandom.self_init tt;; multi_test test_swap).
+
+Separate Extraction run_test.
